README.txt
@@ -3,4 +3,8 @@
 Directory structure:
 
   src      Source files
+    x86    x86-specific definitions and results
+    spred  predicates on state
+    opred  predicates on observables (input and output traces)
+    triple total Hoare triple used for proving properties of monadic semantics    
   doc      Documentation (under construction)
